Finish external_path -> path rename

fstar/MLS.TreeSync.Invariants.ParentHash.Proofs.fst
@@ -682,17 +682,17 @@ let parent_hash_invariant_tree_add #bytes #cb #tkt #l #i t li content =
   parent_hash_invariantP_tree_add t li content;
   parent_hash_invariant_prop2bool (tree_add t li content)
 
-(*** Parent-hash invariant: applying external path ***)
+(*** Parent-hash invariant: applying path ***)
 
 val find_parent_hash_link_aux: #bytes:Type0 -> {|crypto_bytes bytes|} -> #tkt:treekem_types bytes -> #l:nat -> #i:tree_index l -> #li:leaf_index l i -> t:treesync bytes tkt l i -> p:pathsync bytes tkt l i li -> parent_parent_hash:mls_bytes bytes -> Pure (lu:nat & iu:tree_index lu & treesync bytes tkt lu iu)
-  (requires apply_external_path_aux_pre t p (length #bytes parent_parent_hash))
+  (requires apply_path_aux_pre t p (length #bytes parent_parent_hash))
   (ensures fun _ -> True)
 let rec find_parent_hash_link_aux #bytes #cb #tkt #l #i #li t p parent_parent_hash =
   match t, p with
   | TLeaf _, PLeaf _ ->
-    (|l, i, apply_external_path_aux t p parent_parent_hash|)
+    (|l, i, apply_path_aux t p parent_parent_hash|)
   | TNode _ _ _, PNode (Some _) _ -> (
-    (|l, i, apply_external_path_aux t p parent_parent_hash|)
+    (|l, i, apply_path_aux t p parent_parent_hash|)
   )
   | TNode _ left right, PNode None p_next -> (
     if is_left_leaf li then
@@ -709,7 +709,7 @@ let path_node_not_blank #bytes #cb #tkt #l #i #li p =
   | _ -> false
 
 val find_parent_hash_link: #bytes:Type0 -> {|crypto_bytes bytes|} -> #tkt:treekem_types bytes -> #l:pos -> #i:tree_index l -> #li:leaf_index l i -> t:treesync bytes tkt l i -> p:pathsync bytes tkt l i li{path_node_not_blank p} -> parent_parent_hash:mls_bytes bytes -> Pure (lu:nat & iu:tree_index lu & treesync bytes tkt lu iu)
-  (requires apply_external_path_aux_pre t p (length #bytes parent_parent_hash))
+  (requires apply_path_aux_pre t p (length #bytes parent_parent_hash))
   (ensures fun _ -> True)
 let find_parent_hash_link #bytes #cb #tkt #l #i #li t p parent_parent_hash =
   match t, p with
@@ -722,11 +722,11 @@ let find_parent_hash_link #bytes #cb #tkt #l #i #li t p parent_parent_hash =
       find_parent_hash_link_aux right p_next new_parent_parent_hash
   )
 
-val external_path_is_parent_hash_valid_aux: #bytes:Type0 -> {|crypto_bytes bytes|} -> #tkt:treekem_types bytes -> #l:nat -> #i:tree_index l -> #li:leaf_index l i -> treesync bytes tkt l i -> pathsync bytes tkt l i li -> mls_bytes bytes -> bool
-let external_path_is_parent_hash_valid_aux #bytes #cb #tkt #l #i #li t p parent_parent_hash =
-  let new_lp = get_external_path_leaf p in
-  compute_leaf_parent_hash_from_external_path_pre t p (length #bytes parent_parent_hash) && (
-  let computed_parent_hash = compute_leaf_parent_hash_from_external_path t p parent_parent_hash in
+val path_is_parent_hash_valid_aux: #bytes:Type0 -> {|crypto_bytes bytes|} -> #tkt:treekem_types bytes -> #l:nat -> #i:tree_index l -> #li:leaf_index l i -> treesync bytes tkt l i -> pathsync bytes tkt l i li -> mls_bytes bytes -> bool
+let path_is_parent_hash_valid_aux #bytes #cb #tkt #l #i #li t p parent_parent_hash =
+  let new_lp = get_path_leaf p in
+  compute_leaf_parent_hash_from_path_pre t p (length #bytes parent_parent_hash) && (
+  let computed_parent_hash = compute_leaf_parent_hash_from_path t p parent_parent_hash in
   (new_lp.data.source = LNS_commit () && (new_lp.data.parent_hash <: bytes) = computed_parent_hash)
   )
 
@@ -744,15 +744,15 @@ let rec is_tree_empty_implies_empty_resolution #bytes #bl #tkt #l #i t =
 #push-options "--z3rlimit 100"
 //Properties that are just (almost) trivial induction
 val find_parent_hash_link_aux_misc_properties: #bytes:Type0 -> {|crypto_bytes bytes|} -> #tkt:treekem_types bytes -> #l:nat -> #i:tree_index l -> #li:leaf_index l i -> t:treesync bytes tkt l i -> p:pathsync bytes tkt l i li -> parent_parent_hash:mls_bytes bytes -> Lemma
-  (requires external_path_is_parent_hash_valid_aux t p parent_parent_hash /\ external_path_is_filter_valid t p /\ apply_external_path_aux_pre t p (length #bytes parent_parent_hash))
+  (requires path_is_parent_hash_valid_aux t p parent_parent_hash /\ path_is_filter_valid t p /\ apply_path_aux_pre t p (length #bytes parent_parent_hash))
   (ensures (
     let (|lu, iu, u|) = find_parent_hash_link_aux t p parent_parent_hash in
     lu <= l /\
     leaf_index_inside l i iu /\
     node_has_parent_hash u /\
-    is_subtree_of u (apply_external_path_aux t p parent_parent_hash) /\
+    is_subtree_of u (apply_path_aux t p parent_parent_hash) /\
     get_parent_hash_of u == parent_parent_hash /\
-    resolution (apply_external_path_aux t p parent_parent_hash) == [(|lu, iu|)] /\
+    resolution (apply_path_aux t p parent_parent_hash) == [(|lu, iu|)] /\
     True
   ))
 let rec find_parent_hash_link_aux_misc_properties #bytes #cb #tkt #l #i #li t p parent_parent_hash =
@@ -773,13 +773,13 @@ let rec find_parent_hash_link_aux_misc_properties #bytes #cb #tkt #l #i #li t p 
 
 #push-options "--z3rlimit 100"
 val find_parent_hash_link_misc_properties: #bytes:Type0 -> {|crypto_bytes bytes|} -> #tkt:treekem_types bytes -> #l:pos -> #i:tree_index l -> #li:leaf_index l i -> t:treesync bytes tkt l i -> p:pathsync bytes tkt l i li{path_node_not_blank p} -> parent_parent_hash:mls_bytes bytes -> Lemma
-  (requires external_path_is_parent_hash_valid_aux t p parent_parent_hash /\ external_path_is_filter_valid t p /\ apply_external_path_aux_pre t p (length #bytes parent_parent_hash))
+  (requires path_is_parent_hash_valid_aux t p parent_parent_hash /\ path_is_filter_valid t p /\ apply_path_aux_pre t p (length #bytes parent_parent_hash))
   (ensures (
     let (|lu, iu, u|) = find_parent_hash_link t p parent_parent_hash in
     lu < l /\
     leaf_index_inside l i iu /\
     node_has_parent_hash u /\
-    is_subtree_of u (apply_external_path_aux t p parent_parent_hash)
+    is_subtree_of u (apply_path_aux t p parent_parent_hash)
   ))
 let find_parent_hash_link_misc_properties #bytes #cb #tkt #l #i #li t p parent_parent_hash =
   match t, p with
@@ -795,11 +795,11 @@ let find_parent_hash_link_misc_properties #bytes #cb #tkt #l #i #li t p parent_p
 
 #push-options "--fuel 2 --z3rlimit 100"
 val find_parent_hash_link_last_update: #bytes:Type0 -> {|crypto_bytes bytes|} -> #tkt:treekem_types bytes -> #l:pos -> #i:tree_index l -> #li:leaf_index l i -> t:treesync bytes tkt l i -> p:pathsync bytes tkt l i li{path_node_not_blank p} -> parent_parent_hash:mls_bytes bytes -> Lemma
-  (requires external_path_is_parent_hash_valid_aux t p parent_parent_hash /\ external_path_is_filter_valid t p /\ apply_external_path_aux_pre t p (length #bytes parent_parent_hash))
+  (requires path_is_parent_hash_valid_aux t p parent_parent_hash /\ path_is_filter_valid t p /\ apply_path_aux_pre t p (length #bytes parent_parent_hash))
   (ensures (
     find_parent_hash_link_misc_properties t p parent_parent_hash;
     let (|lu, iu, u|) = find_parent_hash_link t p parent_parent_hash in
-    last_update_correct u (apply_external_path_aux t p parent_parent_hash)
+    last_update_correct u (apply_path_aux t p parent_parent_hash)
   ))
 let find_parent_hash_link_last_update #bytes #cb #tkt #l #i #li t p parent_parent_hash =
   find_parent_hash_link_misc_properties t p parent_parent_hash;
@@ -836,11 +836,11 @@ let rec un_add_empty #bytes #tkt #l #i t =
     | Some content -> un_add_empty_lemma content.unmerged_leaves
 
 val find_parent_hash_link_parent_hash: #bytes:Type0 -> {|crypto_bytes bytes|} -> #tkt:treekem_types bytes -> #l:pos -> #i:tree_index l -> #li:leaf_index l i -> t:treesync bytes tkt l i -> p:pathsync bytes tkt l i li{path_node_not_blank p} -> parent_parent_hash:mls_bytes bytes -> Lemma
-  (requires external_path_is_parent_hash_valid_aux t p parent_parent_hash /\ external_path_is_filter_valid t p /\ apply_external_path_aux_pre t p (length #bytes parent_parent_hash))
+  (requires path_is_parent_hash_valid_aux t p parent_parent_hash /\ path_is_filter_valid t p /\ apply_path_aux_pre t p (length #bytes parent_parent_hash))
   (ensures (
     find_parent_hash_link_misc_properties t p parent_parent_hash;
     let (|lu, iu, u|) = find_parent_hash_link t p parent_parent_hash in
-    parent_hash_correct u (apply_external_path_aux t p parent_parent_hash)
+    parent_hash_correct u (apply_path_aux t p parent_parent_hash)
   ))
 let find_parent_hash_link_parent_hash #bytes #cb #tkt #l #i #li t p parent_parent_hash =
   match t, p with
@@ -855,23 +855,23 @@ let find_parent_hash_link_parent_hash #bytes #cb #tkt #l #i #li t p parent_paren
   )
 
 #push-options "--z3rlimit 100"
-val parent_hash_invariantP_apply_external_path_aux: #bytes:Type0 -> {|crypto_bytes bytes|} -> #tkt:treekem_types bytes -> #l:nat -> #i:tree_index l -> #li:leaf_index l i -> t:treesync bytes tkt l i -> p:pathsync bytes tkt l i li -> parent_parent_hash:mls_bytes bytes -> Lemma
-  (requires parent_hash_invariantP t /\ external_path_is_parent_hash_valid_aux t p parent_parent_hash /\ external_path_is_filter_valid t p /\ apply_external_path_aux_pre t p (length #bytes parent_parent_hash))
-  (ensures parent_hash_invariantP (apply_external_path_aux t p parent_parent_hash))
-let rec parent_hash_invariantP_apply_external_path_aux #bytes #cb #tkt #l #i #li t p parent_parent_hash =
+val parent_hash_invariantP_apply_path_aux: #bytes:Type0 -> {|crypto_bytes bytes|} -> #tkt:treekem_types bytes -> #l:nat -> #i:tree_index l -> #li:leaf_index l i -> t:treesync bytes tkt l i -> p:pathsync bytes tkt l i li -> parent_parent_hash:mls_bytes bytes -> Lemma
+  (requires parent_hash_invariantP t /\ path_is_parent_hash_valid_aux t p parent_parent_hash /\ path_is_filter_valid t p /\ apply_path_aux_pre t p (length #bytes parent_parent_hash))
+  (ensures parent_hash_invariantP (apply_path_aux t p parent_parent_hash))
+let rec parent_hash_invariantP_apply_path_aux #bytes #cb #tkt #l #i #li t p parent_parent_hash =
   match t, p with
   | TLeaf content, PLeaf _ -> ()
   | TNode opt_content left right, PNode opt_ext_content p_next ->
     let (child, sibling) = get_child_sibling t li in
     let (_, new_parent_parent_hash) = compute_new_np_and_ph opt_ext_content sibling parent_parent_hash in
-    (if is_left_leaf li then parent_hash_invariantP_apply_external_path_aux left p_next new_parent_parent_hash
-    else parent_hash_invariantP_apply_external_path_aux right p_next new_parent_parent_hash);
+    (if is_left_leaf li then parent_hash_invariantP_apply_path_aux left p_next new_parent_parent_hash
+    else parent_hash_invariantP_apply_path_aux right p_next new_parent_parent_hash);
     match opt_ext_content with
     | None -> ()
     | Some _ -> (
       find_parent_hash_link_misc_properties t p parent_parent_hash;
       let (|lu, iu, u|) = find_parent_hash_link t p parent_parent_hash in
-      node_has_parent_hash_linkP_intro (apply_external_path_aux t p parent_parent_hash) u () () () () (
+      node_has_parent_hash_linkP_intro (apply_path_aux t p parent_parent_hash) u () () () () (
         find_parent_hash_link_last_update t p parent_parent_hash
       ) (
         find_parent_hash_link_parent_hash t p parent_parent_hash
@@ -879,10 +879,10 @@ let rec parent_hash_invariantP_apply_external_path_aux #bytes #cb #tkt #l #i #li
     )
 #pop-options
 
-val parent_hash_invariant_apply_external_path: #bytes:Type0 -> {|crypto_bytes bytes|} -> #tkt:treekem_types bytes -> #l:nat -> #li:leaf_index l 0 -> t:treesync bytes tkt l 0 -> p:pathsync bytes tkt l 0 li -> Lemma
-  (requires parent_hash_invariant t /\ external_path_is_parent_hash_valid t p /\ external_path_is_filter_valid t p /\ apply_external_path_pre t p)
-  (ensures parent_hash_invariant (apply_external_path t p))
-let parent_hash_invariant_apply_external_path #bytes #cb #tkt #l #li t p =
+val parent_hash_invariant_apply_path: #bytes:Type0 -> {|crypto_bytes bytes|} -> #tkt:treekem_types bytes -> #l:nat -> #li:leaf_index l 0 -> t:treesync bytes tkt l 0 -> p:pathsync bytes tkt l 0 li -> Lemma
+  (requires parent_hash_invariant t /\ path_is_parent_hash_valid t p /\ path_is_filter_valid t p /\ apply_path_pre t p)
+  (ensures parent_hash_invariant (apply_path t p))
+let parent_hash_invariant_apply_path #bytes #cb #tkt #l #li t p =
   parent_hash_invariant_bool2prop t;
-  parent_hash_invariantP_apply_external_path_aux t p (root_parent_hash #bytes);
-  parent_hash_invariant_prop2bool (apply_external_path t p)
+  parent_hash_invariantP_apply_path_aux t p (root_parent_hash #bytes);
+  parent_hash_invariant_prop2bool (apply_path t p)
