fstar/MLS.TreeSync.Invariants.UnmergedLeaves.Proofs.fst
@@ -115,27 +115,27 @@ let rec unmerged_leaves_ok_tree_add #bytes #bl #tkt #l #i t li content =
     )
   )
 
-(*** External path ***)
+(*** Apply path ***)
 
-val unmerged_leaves_ok_apply_external_path_aux: #bytes:Type0 -> {|crypto_bytes bytes|} -> #tkt:treekem_types bytes -> #l:nat -> #i:tree_index l -> #li:leaf_index l i -> t:treesync bytes tkt l i -> p:pathsync bytes tkt l i li -> parent_parent_hash:mls_bytes bytes -> Lemma
-  (requires apply_external_path_aux_pre #bytes t p (length #bytes parent_parent_hash) /\ unmerged_leaves_ok t)
-  (ensures unmerged_leaves_ok (apply_external_path_aux t p parent_parent_hash))
-let rec unmerged_leaves_ok_apply_external_path_aux #bytes #cb #tkt #l #i #li t p parent_parent_hash =
+val unmerged_leaves_ok_apply_path_aux: #bytes:Type0 -> {|crypto_bytes bytes|} -> #tkt:treekem_types bytes -> #l:nat -> #i:tree_index l -> #li:leaf_index l i -> t:treesync bytes tkt l i -> p:pathsync bytes tkt l i li -> parent_parent_hash:mls_bytes bytes -> Lemma
+  (requires apply_path_aux_pre #bytes t p (length #bytes parent_parent_hash) /\ unmerged_leaves_ok t)
+  (ensures unmerged_leaves_ok (apply_path_aux t p parent_parent_hash))
+let rec unmerged_leaves_ok_apply_path_aux #bytes #cb #tkt #l #i #li t p parent_parent_hash =
   match t, p with
   | TLeaf _, PLeaf ext_content -> ()
   | TNode _ left right, PNode opt_ext_content p_next ->
     let (child, sibling) = get_child_sibling t li in
     let (new_opt_content, new_parent_parent_hash) = compute_new_np_and_ph opt_ext_content sibling parent_parent_hash in
     if is_left_leaf li then
-      unmerged_leaves_ok_apply_external_path_aux left p_next new_parent_parent_hash
+      unmerged_leaves_ok_apply_path_aux left p_next new_parent_parent_hash
     else
-      unmerged_leaves_ok_apply_external_path_aux right p_next new_parent_parent_hash
+      unmerged_leaves_ok_apply_path_aux right p_next new_parent_parent_hash
 
-val unmerged_leaves_ok_apply_external_path: #bytes:Type0 -> {|crypto_bytes bytes|} -> #tkt:treekem_types bytes -> #l:nat -> #li:leaf_index l 0 -> t:treesync bytes tkt l 0 -> p:pathsync bytes tkt l 0 li -> Lemma
-  (requires apply_external_path_pre #bytes t p /\ unmerged_leaves_ok t)
-  (ensures unmerged_leaves_ok (apply_external_path t p))
-let unmerged_leaves_ok_apply_external_path #bytes #cb #tkt #l #li t p =
-  unmerged_leaves_ok_apply_external_path_aux t p (root_parent_hash #bytes)
+val unmerged_leaves_ok_apply_path: #bytes:Type0 -> {|crypto_bytes bytes|} -> #tkt:treekem_types bytes -> #l:nat -> #li:leaf_index l 0 -> t:treesync bytes tkt l 0 -> p:pathsync bytes tkt l 0 li -> Lemma
+  (requires apply_path_pre #bytes t p /\ unmerged_leaves_ok t)
+  (ensures unmerged_leaves_ok (apply_path t p))
+let unmerged_leaves_ok_apply_path #bytes #cb #tkt #l #li t p =
+  unmerged_leaves_ok_apply_path_aux t p (root_parent_hash #bytes)
 
 (*** Un-add ***)
 
